unique-refs: extended syntax with VReference value, fixed all proofs

src/FrameStack/LogRel.v
@@ -74,6 +74,7 @@ Fixpoint Vrel_rec (n : nat)
   | VNil, VNil => True
   | VLit l, VLit l' => l = l'
   | VPid p, VPid p' => True
+  | VReference p, VReference p' => p = p'
   | VCons hd tl, VCons hd' tl' => Vrel_rec n Vrel hd hd' /\ Vrel_rec n Vrel tl tl'
   | VTuple l, VTuple l' =>
     (fix go l l' :=
@@ -667,6 +668,7 @@ Lemma Vrel_possibilities : forall {n v1 v2},
   (v1 = VNil /\ v2 = VNil) \/
   (exists n, v1 = VLit n /\ v2 = VLit n) \/
   (exists p1 p2, v1 = VPid p1 /\ v2 = VPid p2) \/
+  (exists p1 p2, v1 = VReference p1 /\ v2 = VReference p2) \/
   (exists v11 v12 v21 v22, v1 = VCons v11 v12 /\ v2 = VCons v21 v22) \/
   (exists l l', v1 = VTuple l /\ v2 = VTuple l') \/
   (exists l l', v1 = VMap l /\ v2 = VMap l') \/
@@ -680,7 +682,8 @@ Proof.
   * right. right. right. left. repeat eexists.
   * right. right. right. right. left. repeat eexists.
   * right. right. right. right. right. left. repeat eexists.
-  * right. right. right. right. right. right. repeat eexists.
+  * right. right. right. right. right. right. left. repeat eexists.
+  * right. right. right. right. right. right. right. repeat eexists.
 Qed.
 
 Ltac Vrel_possibilities H0 :=
@@ -755,6 +758,7 @@ Lemma Vrel_ind :
   (HNil : P VNil VNil)
   (HLit : forall l, P (VLit l) (VLit l))
   (HPid : forall p1 p2, P (VPid p1) (VPid p2))
+  (HReference : forall p1 p2, P (VReference p1) (VReference p2))
   (HClos : forall ext ident vl e ext' ident' e', P (VClos ext ident vl e) (VClos ext' ident' vl e'))
   (HCons : forall v1 v2 v1' v2', P v1 v1' -> P v2 v2' -> P (VCons v1 v2) (VCons v1' v2'))
   (HTuple : forall l l', list_biforall P l l' -> P (VTuple l) (VTuple l'))
@@ -762,7 +766,7 @@ Lemma Vrel_ind :
   forall {m} v1 v2 (IH: Vrel m v1 v2),
   P v1 v2.
 Proof.
-  intros ? ? ? ? ? ? ? ? ?. valinduction; try destruct v2; intros.
+  intros ? ? ? ? ? ? ? ? ? ?. valinduction; try destruct v2; intros.
   all: try rewrite Vrel_Fix_eq in IH.
   all: try destruct IH as [IHv1 [IHv2 IH]]; try inv IH; auto.
   all: try destruct_hyps; try contradiction.
